Normalization/LF_Complete.v
@@ -14,6 +14,16 @@ induction M; intros; inversion H; subst;
 eauto using lc_t_n_LF.
 Qed.
 
+Lemma closed_t_addition_LF:
+forall M n m,
+  lc_t_n_LF n M -> lc_t_n_LF (n + m) M.
+intros; induction m;
+[ replace (n+0) with n by auto |
+  replace (n + S m) with (S (n+m)) by auto] ;
+try apply closed_t_succ_LF;
+assumption.
+Qed.
+
 Lemma lc_t_subst_t_LF_free:
 forall M N n v,
   lc_t_n_LF n N ->
@@ -47,15 +57,12 @@ apply lc_t_subst_t_LF_bound; auto.
 eapply IHM1; eauto.
 eapply IHM; eauto.
 eapply IHM; eauto.
+(*constructor; auto. *)
 unfold open_LF; apply lc_t_subst_t_LF_bound; auto.
 eapply IHM1; eauto.
+(* constructor; auto. apply closed_t_succ_LF; auto. *)
 Qed.
 
-Require Export Relations.
-Definition multisteps := clos_refl_trans_1n _ step_LF.
-Notation " M |->* N " := (multisteps M N) (at level 70).
-
-(*
 Definition normal_form (M: te_LF) := value_LF M.
 
 Inductive neutral_LF: te_LF -> Prop :=
@@ -63,7 +70,7 @@ Inductive neutral_LF: te_LF -> Prop :=
 | nAppl: forall M N, neutral_LF (appl_LF M N)
 | nUnbox: forall M, neutral_LF (unbox_LF M)
 | nHere: forall M, neutral_LF M -> neutral_LF (here_LF M)
-| nLetd: forall M N, neutral_LF (letdia_LF M N)
+| nLetd: forall M N A, neutral_LF (letdia_LF A M N)
 .
 
 Lemma value_no_step_LF:
@@ -71,7 +78,7 @@ forall M,
   value_LF M ->
   forall N , ~ M |-> N.
 induction M; intros; intro;
-try inversion H; inversion H0; subst;
+try inversion H; inversion H0; subst; try inversion H2;
 eapply IHM; eauto.
 Qed.
 
@@ -85,23 +92,110 @@ right;
 constructor.
 Qed.
 
-Inductive SN: te_LF -> Prop :=
-| val_SN: forall M, value_LF M -> SN M
-| step_SN: forall M,
-             (forall N, M |-> N -> SN N) ->
-             SN M.
-*)
+Require Export Relations.
+Definition multisteps := clos_refl_trans_1n _ step_LF.
+Notation " M |->* N " := (multisteps M N) (at level 70).
 
-Lemma value_no_step_LF:
-forall M,
-  value_LF M ->
-  forall N , ~ M |-> N.
-induction M; intros; intro;
-try inversion H; inversion H0; subst;
-eapply IHM; eauto.
+
+Definition WT' (M: te_LF) :=
+  exists V, value_LF V /\ M |->* V.
+
+(* FIXME: WT' would be more elegant *)
+Inductive WT: te_LF -> Prop :=
+| val_WT: forall V, value_LF V -> WT V
+| step_WT: forall M, (exists V, value_LF V /\ steps_LF M V) -> WT M
+.
+
+Lemma step_LF_unique:
+forall M N1 N2,
+  M |-> N1 ->
+  M |-> N2 ->
+  N1 = N2.
+induction M; intros; inversion H; inversion H0; subst; auto.
+inversion H6; subst; auto.
+inversion H11.
+inversion H6.
+specialize IHM1 with M' M'0; rewrite IHM1; auto.
+inversion H4; subst; auto.
+inversion H6.
+inversion H3.
+specialize IHM with M' M'0; rewrite IHM; auto.
+specialize IHM with M' M'0; rewrite IHM; auto.
+inversion H9; subst; auto.
+inversion H14; subst. apply value_no_step_LF in H3; auto; contradiction.
+inversion H7; subst. apply value_no_step_LF in H3; auto; contradiction.
+specialize IHM1 with M' M'0; rewrite IHM1; auto.
 Qed.
 
-Definition WT (M: te_LF) := exists V, value_LF V /\ M |->* V.
+Theorem WT_step:
+forall M M',
+  WT M ->
+  M |-> M' ->
+  WT M'.
+intros; inversion H; subst.
+apply value_no_step_LF with (N:=M') in H1; contradiction.
+destruct H1 as (V, (H1, H2)).
+inversion H2; subst.
+apply step_LF_unique with (N1:=V) in H0; subst; auto. constructor; auto.
+apply step_WT; exists V; split; auto.
+apply step_LF_unique with (N1:=M'0) in H0; subst; auto.
+Qed.
+
+Lemma WT_step_back:
+forall M N,
+  WT N ->
+  M |-> N ->
+  WT M.
+intros; inversion H; subst.
+apply step_WT; exists N; split; auto; constructor; auto.
+destruct H1 as (V, (H1, H2)); apply step_WT; exists V; split; auto.
+apply multi_step_LF with (M':=N); auto.
+Qed.
+
+Lemma here_val:
+forall M V,
+  value_LF V -> steps_LF (here_LF M) V ->
+  exists M', V = here_LF M'.
+intros; remember (here_LF M) as M0; generalize dependent M.
+induction H0; intros; subst.
+inversion H0; subst. eexists; eauto.
+inversion H0; subst.
+apply IHsteps_LF with (M:=M'0); auto.
+Qed.
+
+Lemma WT_here:
+forall M,
+  lc_t_LF M ->
+  (WT M <-> WT (here_LF M)).
+split.
+intros; inversion H0; subst.
+constructor; constructor; auto.
+destruct H1 as (V, (H1, H2)).
+apply step_WT; exists (here_LF V); split.
+constructor; auto.
+induction H2; intros; subst.
+  constructor; constructor; auto.
+  apply multi_step_LF with (here_LF M').
+    constructor; auto.
+    apply IHsteps_LF; auto.
+    apply lc_t_step_LF in H2; auto.
+    apply WT_step in H2; auto.
+intros. remember (here_LF M) as T; generalize dependent M.
+induction H0; intros; subst.
+inversion H; constructor; subst; auto.
+destruct H as (V, (H, H1)).
+assert ( steps_LF (here_LF M0) V) by auto.
+apply here_val in H1; auto; destruct H1; subst.
+apply step_WT; exists x; split; inversion H; subst; auto.
+remember (here_LF M0) as hm; remember (here_LF x) as hx; generalize dependent x;
+generalize dependent M0; induction H2; intros; subst.
+inversion H0; subst; constructor; auto.
+inversion H0; subst.
+apply multi_step_LF with M'0; auto. apply IHsteps_LF; auto.
+apply lc_t_step_LF in H6; auto.
+Qed.
+
+Hint Resolve WT_step.
 
 Inductive Cont :=
 | IdK: ty -> Cont
@@ -121,7 +215,7 @@ Inductive ContTyping: Cont -> ty -> ty -> Prop:=
 Fixpoint ContAppl (K: Cont) (M: te_LF) : te_LF :=
 match K with
 | IdK A => here_LF M
-| ConsK K' N A B => ContAppl K' (letdia_LF M (here_LF N))
+| ConsK K' N A B => ContAppl K' (here_LF (letdia_LF A M N))
 end.
 
 Inductive ContLC: Cont -> Prop :=
@@ -139,19 +233,11 @@ forall K M M',
 induction K; intros; simpl in *.
 constructor; auto.
 inversion H; subst.
-assert ((letdia_LF M (here_LF t)) |-> (letdia_LF M' (here_LF t))).
+assert (here_LF (letdia_LF t0 M t) |-> here_LF (letdia_LF t0 M' t)).
    constructor; auto; constructor; auto.
 apply IHK in H2; auto.
 constructor; auto; constructor; auto.
 Qed.
-
-Inductive neutral_LF: te_LF -> Prop :=
-| nHyp: forall n, neutral_LF (hyp_LF n)
-| nAppl: forall M N, neutral_LF (appl_LF M N)
-| nUnbox: forall M, neutral_LF (unbox_LF M)
-| nHere: forall M, neutral_LF M -> neutral_LF (here_LF M)
-| nLetd: forall M N, neutral_LF (letdia_LF M N)
-.
 
 Lemma neutral_ContAppl:
 forall K M,
@@ -175,53 +261,40 @@ forall K M,
   value_LF M /\ exists A, K = IdK A.
 induction K; intros; simpl in *.
 inversion H; subst; split; auto; eexists; auto.
-assert (neutral_LF (ContAppl K (letdia_LF M (here_LF t)))).
-apply neutral_ContAppl; constructor.
+assert (neutral_LF (ContAppl K (here_LF (letdia_LF t0 M t)))).
+apply neutral_ContAppl; constructor; constructor.
 apply neutral_not_value_LF in H0; contradiction.
 Qed.
 
 Fixpoint Red (M: te_LF) (A: ty) : Prop :=
+let RedCont K A :=
+    (forall V, Red V A -> lc_t_LF V ->
+               WT (ContAppl K (here_LF V))) in
 match A with
 | tvar => WT M
 | tarrow A1 A2 =>
+  WT M /\
   forall N
          (H_lc: lc_t_LF N)
          (HRed: Red N A1),
-    Red (appl_LF M N) A2
-| tbox A1 => Red (unbox_LF M) A1
+    forall K,
+      ContLC K ->
+      RedCont K A2 ->
+    WT (ContAppl K (here_LF (appl_LF M N)))
+
+| tbox A1 => WT M /\
+             forall K,
+               ContLC K ->
+               RedCont K A1 ->
+               WT (ContAppl K (here_LF (unbox_LF M)))
 | tdia A1 =>
-  forall K B,
+  forall K,
     ContLC K ->
-    ContTyping K A1 B ->
-(* Definition of reducible continuation is embedded *)
-    (forall V, Red V A1 -> lc_t_LF V ->
-               WT (ContAppl K (here_LF V))) ->
+    RedCont K A1 ->
     WT (ContAppl K M)
 end.
 
-Lemma step_LF_unique:
-forall M N1 N2,
-  M |-> N1 ->
-  M |-> N2 ->
-  N1 = N2.
-induction M; intros; inversion H; inversion H0; subst; auto.
-inversion H6; subst; auto.
-inversion H11.
-inversion H6.
-specialize IHM1 with M' M'0; rewrite IHM1; auto.
-inversion H4; subst; auto.
-inversion H6.
-inversion H3.
-specialize IHM with M' M'0; rewrite IHM; auto.
-specialize IHM with M' M'0; rewrite IHM; auto.
-inversion H7; subst; auto.
-inversion H12; subst. apply value_no_step_LF in H5; auto; contradiction.
-inversion H6; subst. apply value_no_step_LF in H5; auto; contradiction.
-specialize IHM1 with M' M'0; rewrite IHM1; auto.
-Qed.
-
-Definition ContReducible K A B:=
-  ContTyping K A B ->
+Definition RedCont K A:=
     (forall V, Red V A -> lc_t_LF V ->
                WT (ContAppl K (here_LF V))).
 
@@ -234,30 +307,28 @@ forall A M M'
   Red M' A.
 induction A; intros; simpl in *; intros.
 (* base type *)
-unfold WT in *; destruct HRed as (V, (H0, H1)).
-exists V; split; auto.
-inversion H1; subst. apply value_no_step_LF with (N:=M') in H0; contradiction.
-assert (y = M'); subst; auto.
-apply step_LF_unique with M; auto.
+eauto.
 (* arrow type *)
-apply IHA2 with (M:=appl_LF M N); auto.
-constructor; auto.
-constructor; auto.
-(* box type *)
-apply IHA with (M:=unbox_LF M); auto; constructor; eauto.
-(* dia type *)
-unfold WT in *.
-specialize HRed with K B.
-assert (ContLC K) by auto;
-apply HRed in H; auto.
-destruct H as (V, (H, H3)); exists V; split; auto.
-inversion H3; subst.
-apply value_ContAppl in H; destruct H.
-apply value_no_step_LF in HStep; auto; contradiction.
-assert (ContAppl K M |-> ContAppl K M').
+destruct HRed; split; eauto; intros.
+apply WT_step with (M:=ContAppl K (here_LF (appl_LF M N))).
+apply H0; auto.
 apply Step_KApplStep; auto.
-assert (ContAppl K M' = y); subst; auto.
-apply step_LF_unique with (ContAppl K M); auto.
+constructor; constructor; auto.
+constructor; constructor; auto.
+(* box type *)
+destruct HRed; split; eauto; intros.
+apply WT_step with (M:=ContAppl K (here_LF (unbox_LF M))).
+apply H0; auto.
+apply Step_KApplStep; auto.
+constructor; constructor; auto.
+constructor; constructor; auto.
+(* dia type *)
+specialize HRed with K; assert (ContLC K) by auto;
+apply HRed in H; auto; inversion H; subst.
+apply value_ContAppl in H2; destruct H2; destruct H3; subst; simpl in *;
+apply value_no_step_LF in HStep; auto; contradiction.
+assert (ContAppl K M |-> ContAppl K M') by (apply Step_KApplStep; auto);
+destruct H2 as (V, (H2, H5)); eauto.
 Qed.
 
 Lemma head_expansion_star:
@@ -266,11 +337,26 @@ forall A M M'
   (H_lc_t: lc_t_LF M)
   (HStep: M |->* M'),
   Red M' A.
-intros; induction HStep; [ assumption | ].
-apply IHHStep.
-Focus 2.
-apply lc_t_step_LF with x; auto.
-apply property_2 with x; auto.
+intros; induction HStep; [ assumption | ];
+apply IHHStep;
+[apply property_2 with x | apply lc_t_step_LF with x]; auto.
+Qed.
+
+Lemma lc_ContAppl:
+forall K M,
+  ContLC K-> lc_t_LF M -> lc_t_LF (ContAppl K M).
+induction K; intros; simpl in *.
+constructor; auto.
+inversion H; subst.
+apply IHK with (M:=here_LF(letdia_LF t0 M t)) in H3; auto.
+constructor; auto. constructor; auto.
+Qed.
+
+Lemma neutral_not_value:
+forall M,
+  neutral_LF M -> ~ value_LF M.
+induction M; intros; intro; try inversion H0; subst; inversion H; subst;
+apply IHM in H3; contradiction.
 Qed.
 
 Fixpoint find_var (L: list (var * ty * te_LF)) (x:var) :
@@ -280,6 +366,116 @@ match L with
 | (v, A, M) :: L' =>
   if (eq_var_dec x v) then Some (v, A, M) else find_var L' x
 end.
+
+Lemma Mem_find_var:
+  forall L v,
+    Mem v (map fst_ (map fst_ L)) ->
+    exists A M, find_var L v = Some (v, A, M).
+induction L; intros; [ rewrite Mem_nil_eq in *; contradiction | ];
+destruct a; destruct p; rew_map in *; simpl in *.
+subst; rewrite Mem_cons_eq in H.
+destruct (eq_var_dec v v0).
+subst; simpl; exists t0 t; auto.
+destruct H; try contradiction; apply IHL; auto.
+Qed.
+
+Lemma NotMem_find_var:
+  forall L v,
+    ~Mem v (map fst_ (map fst_ L)) ->
+    find_var L v = None.
+induction L; intros; simpl in *; auto;
+destruct a; destruct p; rew_map in *; simpl in *;
+case_if.
+elim H; apply Mem_here.
+apply IHL; intro; elim H;
+rewrite Mem_cons_eq; right; auto.
+Qed.
+
+Lemma find_var_Mem:
+forall L v A M,
+  find_var L v = Some (v, A, M) -> Mem (v, A, M) L.
+induction L; intros; [inversion H; subst | ].
+destruct a; destruct p; simpl in *; case_if.
+inversion H; subst; apply Mem_here.
+rewrite Mem_cons_eq; right; apply IHL; auto.
+Qed.
+
+Fixpoint OkL (L: list (var * ty * te_LF)) U :=
+match L with
+| nil => True
+| (v, A, M) :: L' => ~ Mem v U /\ OkL L' (v::U)
+end.
+
+Lemma OkL_permut:
+forall L U1 U2,
+  U1 *=* U2 ->
+  OkL L U1 -> OkL L U2.
+induction L; intros; [constructor | destruct a; destruct p];
+inversion H0; subst; constructor.
+intro; elim H1; apply Mem_permut with (l:=U2); [symmetry | ]; auto.
+apply IHL with (U1:=v::U1); auto.
+Qed.
+
+Lemma OkL_weaken:
+forall L U w,
+  OkL L (w::U) -> OkL L U.
+induction L; intros; simpl in *; auto; destruct a; destruct p; destruct H;
+split.
+intro; elim H; rewrite Mem_cons_eq; right; auto.
+apply IHL with w. apply OkL_permut with (U1:=v::w::U); auto; permut_simpl.
+Qed.
+
+Lemma OkL_used_notin:
+forall L U x A M,
+  OkL L U ->
+  Mem x U ->
+  ~ Mem (x, A, M) L.
+induction L; intros.
+rewrite Mem_nil_eq; tauto.
+intro; destruct a; destruct p; rewrite Mem_cons_eq in *; inversion H; subst;
+destruct H1.
+inversion H1; subst; contradiction.
+specialize IHL with U x A M.
+apply OkL_weaken in H3; apply IHL in H3; auto.
+Qed.
+
+Lemma OkL_fresh:
+forall L x U,
+  OkL L U->
+  x \notin from_list (map fst_ (map fst_ L)) \u from_list U ->
+  OkL L (x::U).
+induction L; intros; [constructor | destruct a; destruct p];
+simpl in *; destruct H; split.
+intro; elim H; rewrite Mem_cons_eq in *; destruct H2; subst; auto;
+repeat rewrite notin_union in *; destruct H0; destruct H0;
+rew_map; simpl; rewrite from_list_cons; rewrite in_union; left;
+rewrite in_singleton; auto.
+apply OkL_permut with (U1:=x::v::U); [permut_simpl | apply IHL]; auto.
+rew_map in *; simpl in *;
+repeat rewrite from_list_cons in *; repeat rewrite notin_union in *;
+simpl in *; destruct H0; destruct H0; split; auto.
+Qed.
+
+Lemma Mem_find_var_type:
+  forall L v A,
+    OkL L nil ->
+    Mem (v, A) (map fst_ L) ->
+    {M | find_var L v = Some (v, A, M)}.
+induction L; intros; [ rewrite Mem_nil_eq in *; contradiction | ];
+destruct a; destruct p; rew_map in *; simpl in *; destruct H.
+subst; apply Mem_cons_spec in H0.
+case_if.
+destruct H0.
+inversion e; subst; exists t; auto.
+destruct IHL with v0 A; auto.
+apply OkL_weaken in H1; auto.
+apply find_var_Mem in e.
+apply OkL_used_notin with (x:=v0) (A:=A) (M:=x) in H1; [ | apply Mem_here];
+contradiction.
+destruct H0; [inversion e; subst; elim H2; auto | ].
+apply IHL; auto; apply OkL_weaken in H1; auto.
+intros; decide equality. apply eq_ty_dec. apply eq_var_dec.
+Qed.
 
 Fixpoint SL (L: list (var * ty * te_LF)) M :=
 match M with
@@ -295,25 +491,387 @@ match M with
 | box_LF M => box_LF (SL L M)
 | unbox_LF M => unbox_LF (SL L M)
 | here_LF M => here_LF (SL L M)
-| letdia_LF M N => letdia_LF (SL L M) (SL L N)
+| letdia_LF A M N => letdia_LF A (SL L M) (SL L N)
 end.
+
+Lemma lc_SL:
+forall M L n,
+  lc_t_n_LF n M ->
+  (forall a b c, Mem (a,b,c) L -> lc_t_LF c) ->
+  lc_t_n_LF n (SL L M).
+induction M; intros; simpl in *;
+try (inversion H; subst; constructor; eapply IHM; eauto).
+destruct v; inversion H; subst;
+[constructor; auto | ];
+destruct (Mem_dec var (map fst_ (map fst_ L)) v);
+[apply eq_var_dec | apply Mem_find_var in m; destruct m; destruct H1 | ].
+rewrite H1; replace n with (0+n) by omega;
+apply closed_t_addition_LF; apply H0 with v x; apply find_var_Mem; auto.
+rewrite NotMem_find_var; auto.
+inversion H; subst; constructor; [apply IHM1 | apply IHM2]; auto.
+inversion H; subst; constructor; [eapply IHM2 | apply IHM1]; auto.
+Qed.
+
+Lemma SL_hyp:
+forall L G Gamma v A,
+  OkL L nil ->
+  concat (Gamma::G) *=* map fst_ L ->
+  (forall a b c, Mem (a, b, c) L -> Red c b) ->
+  G |= Gamma |- hyp_LF (fte v) ::: A ->
+  Red (SL L (hyp_LF (fte v))) A.
+intros; inversion H2; subst.
+assert (Mem (v, A) (map fst_ L)).
+  apply Mem_permut with (l:=concat (Gamma::G)); auto.
+  rew_concat; rewrite Mem_app_or_eq; left; auto.
+apply Mem_find_var_type in H3; auto. destruct H3.
+simpl; rewrite e; apply H1 with v.
+apply find_var_Mem; auto.
+Qed.
+
+Lemma eq_te_LF_dec:
+forall (M1: te_LF) (M2: te_LF),
+  {M1 = M2} + {M1 <> M2}.
+decide equality.
+apply eq_vte_dec.
+apply eq_ty_dec.
+apply eq_ty_dec.
+Qed.
+
+Lemma SL_bte_subst:
+forall L0 M x k,
+  ~ Mem x (map fst_ (map fst_ L0)) ->
+  (forall v a m, Mem (v, a, m) L0 -> lc_t_LF m) ->
+  [hyp_LF (fte x) // bte k](SL L0 M) =
+  SL L0 [hyp_LF (fte x) // bte k]M.
+induction M; intros; simpl in *;
+try rewrite IHM || (rewrite IHM1; try rewrite IHM2); auto.
+case_if; simpl.
+case_if. rewrite NotMem_find_var; auto.
+destruct v; simpl; repeat case_if; auto.
+destruct (Mem_dec var (map fst_ (map fst_ L0)) v);
+try apply eq_var_dec; [ | rewrite NotMem_find_var]; auto;
+simpl; repeat case_if; auto.
+apply Mem_find_var in m; destruct m as (a, (b, m)); rewrite m; simpl.
+rewrite closed_subst_t_bound_LF with (n:=0); auto; try omega;
+apply H0 with v a; apply find_var_Mem; auto.
+Qed.
+
+Fixpoint FV_L (L: list (var * ty * te_LF)) :=
+match L with
+| nil => \{}
+| (v, A, M) :: L' => used_vars_te_LF M \u FV_L L'
+end.
+
+Lemma notin_FV_notin_elem:
+forall x L,
+  x \notin FV_L L ->
+  forall a b c, Mem (a,b,c) L -> x \notin used_vars_te_LF c.
+induction L; intros; simpl in *.
+rewrite Mem_nil_eq in *; contradiction.
+rewrite Mem_cons_eq in H0; destruct H0; [inversion H0; subst | ].
+rewrite notin_union in H; destruct H; auto.
+destruct a; destruct p; rewrite notin_union in H; destruct H;
+apply IHL with (a:=a0) (b:=b); auto.
+Qed.
+
+Lemma SL_extend:
+forall M L0 x A N,
+  x \notin FV_L L0 ->
+  ~Mem x (map fst_ (map fst_ L0)) ->
+  SL ((x, A, N) :: L0) M =
+  [N // fte x](SL L0 M).
+induction M; intros; simpl in *;
+try rewrite IHM || (rewrite IHM1; try rewrite IHM2); auto.
+destruct v; simpl; repeat case_if; auto.
+rewrite NotMem_find_var; auto; simpl; case_if; auto.
+destruct (Mem_dec var (map fst_ (map fst_ L0)) v);
+try apply eq_var_dec; [ | rewrite NotMem_find_var]; auto;
+simpl; repeat case_if; auto.
+apply Mem_find_var in m; destruct m as (a, (b, m)); rewrite m; simpl.
+rewrite closed_subst_t_free_LF; auto.
+apply notin_FV_notin_elem with L0 v a; eauto.
+apply find_var_Mem; eauto.
+Qed.
+
+Lemma property_1:
+forall A M
+  (H_lc_t: lc_t_LF M),
+  Red M A -> WT M.
+induction A; intros; simpl in *; auto.
+destruct H; auto.
+destruct H; auto.
+assert (WT (ContAppl (IdK A) M)).
+apply H.
+constructor.
+intros; simpl in *. rewrite <- WT_here. rewrite <- WT_here; auto.
+constructor; auto.
+simpl in H0. apply WT_here in H0; auto.
+Qed.
 
 Theorem main_theorem:
 forall G Gamma M A,
   lc_t_LF M ->
   G |= Gamma |- M ::: A ->
  forall L,
+    OkL L nil ->
     concat(Gamma::G) *=* map fst_ L ->
     (forall a b c, Mem (a,b,c) L -> lc_t_LF c) ->
     (forall a b c, Mem (a,b,c) L -> Red c b) ->
-  forall K B,
-    ContTyping K A B ->
-    ContReducible K A B ->
+  forall K,
+    ContLC K ->
+    RedCont K A ->
     WT (ContAppl K (here_LF (SL L M))).
-intros G Gamma M A LC HT; induction HT; unfold ContReducible in *;
+intros G Gamma M A LC HT.
+induction HT; unfold RedCont in *;
 intros; simpl in *.
-Focus 9.
+(* hyp *)
+assert (lc_t_LF (SL L (hyp_LF (fte v)))) by
+  (apply lc_SL; auto; constructor);
+simpl in *;
+remember (match find_var L v with
+           | Some (_, _, M) => M
+           | None => hyp_LF (fte v)
+           end) as M';
+assert (Red M' A)
+  by (subst; apply SL_hyp with G Gamma; auto; constructor; auto);
+apply H5; auto.
+(* lam *)
+apply H6; auto; [split | inversion LC; constructor; apply lc_SL; auto];
+[repeat constructor | intros];
+apply WT_step_back with (N:=ContAppl K0 (here_LF ((SL L0 M) ^t^ N))).
+unfold open_LF in *;
+assert (exists x, x \notin L \u used_vars_te_LF (SL L0 M) \u FV_L L0
+       \u  from_list (map fst_ (map fst_ L0))  \u from_list nil)
+  by apply Fresh; destruct H9;
+rewrite subst_t_neutral_free_LF with (v:=x); auto;
+replace (here_LF [N // fte x]([hyp_LF (fte x) // bte 0](SL L0 M))) with
+(here_LF (SL ((x, A, N) :: L0) ([hyp_LF (fte x) // bte 0]M))).
+apply H0; auto.
+apply lc_t_subst_t_LF_bound.
+ constructor. inversion LC; auto.
+constructor; [ rewrite Mem_nil_eq | apply OkL_fresh]; auto.
+rew_map in *; simpl; rewrite <-  H2; rew_concat; auto.
+intros; rewrite Mem_cons_eq in *; destruct H10.
+inversion H10; subst; auto.
+apply H3 with a b; auto.
+intros; apply Mem_cons_spec in H10. destruct H10.
+inversion e; subst; auto.
+apply H4 with a; auto.
+intros; destruct k; destruct p; destruct k'; destruct p; decide equality.
+apply eq_te_LF_dec. destruct p; destruct a0; decide equality.
+apply eq_ty_dec. apply eq_var_dec.
+rewrite SL_bte_subst; auto. rewrite SL_extend; auto.
+apply notin_Mem; auto.
+apply notin_Mem; auto.
+apply Step_KApplStep; auto.
+repeat constructor; auto; apply lc_SL; auto. inversion LC; auto.
+constructor. repeat constructor; auto; inversion LC; apply lc_SL; auto.
+constructor. apply lc_SL; inversion LC; auto. auto.
+Focus 2.
+(* box *)
+inversion LC; subst;
+apply H4; [ | constructor; apply lc_SL; auto];
+split; [ repeat constructor | intros].
+apply WT_step_back with (N:=ContAppl K0 (here_LF (SL L M))).
+apply IHHT; auto.
+rew_map in *; simpl; rewrite <-  H0; rew_concat; auto.
+apply Step_KApplStep; auto.
+repeat constructor; apply lc_SL; auto.
+constructor. repeat constructor; apply lc_SL; auto.
+constructor; apply lc_SL; auto.
+Focus 4.
+apply H4; [ intros | inversion LC; constructor; apply lc_SL; auto].
+apply IHHT; inversion LC; auto.
+Focus 4.
+apply H5; [ intros | inversion LC; constructor; apply lc_SL; auto].
+apply IHHT; inversion LC; subst; auto.
+rew_map in *; simpl; rewrite <-  H1; rew_concat; auto. permut_simpl.
+replace (Gamma ++ concat G) with (concat (Gamma::G)) by (rew_concat; auto).
+apply PPermut_concat_permut; rewrite <- H; PPermut_LF_simpl.
+Focus 4.
+replace (ContAppl K (here_LF (letdia_LF A (SL L0 M) (SL L0 N)))) with
+(ContAppl (ConsK K (SL L0 N) A B) (SL L0 M)).
+Focus 2. simpl; auto.
+apply WT_here. skip.
+assert (WT (here_LF (ContAppl (ConsK K (SL L0 N) A B) (SL L0 M))) <->
+WT ((ContAppl (ConsK K (SL L0 N) A B) (here_LF (SL L0 M))))).
+skip.
+inversion LC; subst; apply H6; apply IHHT; auto.
+constructor; auto; apply lc_SL; auto.
+intros.
+assert (WT (here_LF (ContAppl (ConsK K (SL L0 N) A B) V)) <->
+WT ((ContAppl (ConsK K (SL L0 N) A B) (here_LF V)))).
+skip.
+apply H9. rewrite <- WT_here. simpl.
+simpl.
 
+
+Focus 2.
+inversion LC; subst.
+assert (WT (ContAppl K (here_LF (SL L M)))).
+apply IHHT; auto; intros; destruct H5.
+assert (WT (ContAppl K (here_LF (unbox_LF V)))).
+apply H8; auto.
+skip.
+<
+
+
+inversion LC; subst.
+
+
+
+
+
+
+
+
+
+remember (here_LF (appl_LF (SL L M) (SL L N))) as HMN.
+generalize dependent M;
+generalize dependent N;
+generalize dependent L;
+generalize dependent A;
+generalize dependent B.
+induction K; intros.
+subst.
+assert (WT (ContAppl (IdK (A ---> B)) (here_LF (SL L M)))).
+apply IHHT1; auto; intros. destruct H4.
+simpl. apply WT_here. constructor; auto.
+simpl. apply WT_here; auto.
+simpl in *.
+apply WT_here. repeat constructor; apply lc_SL; auto.
+apply WT_here. repeat constructor; apply lc_SL; auto.
+skip.
+simpl.
+assert (WT (ContAppl (IdK A) (here_LF (SL L N)))).
+apply IHHT2; auto; intros.
+simpl. apply WT_here. constructor; auto.
+apply WT_here; auto. apply property_1 in H5; auto.
+assert (WT (ContAppl K (here_LF (SL L M)))).
+apply IHHT1; auto; intros. destruct H6.
+
+simpl. apply WT_here. constructor; auto.
+simpl. apply WT_here; auto.
+
+
+assert (Red (SL L M) (A ---> B)).
+simpl in *; split.
+apply WT_here_back. apply lc_SL; auto.
+apply WT_here_back. constructor; apply lc_SL; auto.
+auto.
+intros.
+
+assert (WT (ContAppl (IdK (A ---> B)) (here_LF (SL L M)))).
+apply IHHT1; auto.
+constructor. auto.
+intros. simpl.
+destruct H6.
+Lemma WT_expand:
+forall M A,
+  lc_t_LF M ->
+  WT M ->
+  WT (letdia_LF A (here_LF M) (hyp_LF (bte 0))).
+intros. inversion H0; subst; apply step_WT.
+exists ((hyp_LF (bte 0)) ^t^ M); split;
+[unfold open_LF; simpl; case_if; auto | constructor].
+constructor; auto. constructor; omega.
+destruct H1; destruct H1; exists x; split; auto.
+assert (steps_LF (letdia_LF A (here_LF M) (hyp_LF (bte 0)))
+                 (letdia_LF A (here_LF x) (hyp_LF (bte 0)))).
+remember (here_LF M) as y.
+remember (here_LF x) as x'.
+remember (hyp_LF (bte 0)) as z.
+induction H2.
+constructor; constructor; auto.
+subst; constructor; auto.
+subst; constructor; omega.
+subst; constructor; auto. skip.
+skip.
+Qed.
+simpl.
+apply WT_expand with (A:=A ---> B) in H6.
+replace (appl_LF (SL L M) (SL L N)) with (SL L (appl_LF M N)) by (simpl; auto).
+
+assert (WT (ContAppl (IdK (A ---> B)) (here_LF (SL L M)))).
+apply IHHT1 with (A ---> B); auto. constructor.
+intros; destruct H6; simpl.
+apply WT_here. constructor; auto. apply WT_here; auto.
+
+apply H6; auto; [ | inversion LC; subst; constructor; apply lc_SL; auto];
+split; [constructor; constructor | intros].
+
+(* appl *)
+(* box *)
+(* unbox *)
+(* here *)
+(* get_here *)
+(* letdia *)
+(* letdia_get *)
+
+
+
+
+
+
+
+
+
+
+
+
+
+
+
+
+
+
+
+
+
+
+
+
+
+
+
+
+
+
+
+
+
+
+
+
+
+
+
+
+
+
+
+
+
+
+
+
+
+
+
+
+
+
+
+
+
+
+
+Focus 9.
+apply step_WT; intros.
+
+simpl in *.
+(* here (letdia x = m in n ) -> letdia x = m in here n*)
+(* letdia y = (letdia x = m in n ) in p - > letdia x =m in letdia y= here n in p *)
 
 (*
 Lemma lc_t_subst_t_LF_bound:
@@ -342,11 +900,11 @@ unfold open_LF; apply lc_t_subst_t_LF_bound; auto.
 eapply IHM1; eauto.
 Qed.
 
-Lemma SN_appl:
+Lemma WT_appl:
 forall M N,
   lc_t_LF (appl_LF M N) ->
-  SN (appl_LF M N) ->
-  SN M.
+  WT (appl_LF M N) ->
+  WT M.
 intros;
 remember (appl_LF M N) as T;
 generalize dependent M;
@@ -357,36 +915,36 @@ induction H0; intros; subst;
 destruct H2;
 [ inversion H; subst |
   constructor; auto];
-apply step_SN; intros;
+apply step_WT; intros;
 apply H1 with (N0:=appl_LF N0 N) (N:=N).
 constructor; eauto.
 apply lc_t_step_LF with (M:=appl_LF M0 N); auto; constructor; auto.
 auto.
 Qed.
 
-Lemma SN_box:
+Lemma WT_box:
 forall M,
   lc_t_LF (unbox_LF M) ->
-  SN (unbox_LF M) ->
-  SN M.
+  WT (unbox_LF M) ->
+  WT M.
 intros; remember (unbox_LF M) as T;
 generalize dependent M;
 induction H0; intros; subst;
 [ inversion H0 |
   assert (neutral_LF M0 \/ value_LF M0) by apply neutral_or_value_LF];
 destruct H2; [ inversion H; subst | constructor; auto];
-apply step_SN; intros;
+apply step_WT; intros;
 apply H1 with (N := unbox_LF N).
 constructor; inversion H; auto.
 apply lc_t_step_LF with (M:=unbox_LF M0); auto; constructor; auto.
 auto.
 Qed.
 
-Lemma SN_here:
+Lemma WT_here:
 forall M,
   lc_t_LF (here_LF M) ->
-  SN (here_LF M) ->
-  SN M.
+  WT (here_LF M) ->
+  WT M.
 intros;
 remember (here_LF M) as T;
 generalize dependent M;
@@ -396,18 +954,18 @@ assert (neutral_LF M0 \/ value_LF M0) by apply neutral_or_value_LF.
 destruct H2;
 [ inversion H; subst |
   constructor; auto].
-apply step_SN; intros;
+apply step_WT; intros;
 apply H1 with (N:=here_LF N).
 constructor; eauto.
 apply lc_t_step_LF with (M:=here_LF M0); auto; constructor; auto.
 auto.
 Qed.
 
-Theorem SN_step:
+Theorem WT_step:
 forall M M',
-  SN M ->
+  WT M ->
   M |-> M' ->
-  SN M'.
+  WT M'.
 intros; inversion H; subst.
 apply value_no_step_LF with (N:=M') in H1; contradiction.
 apply H1; auto.
@@ -449,16 +1007,16 @@ apply IHA with (M:=unbox_LF M); auto; constructor; eauto.
 specialize HRed with K B.
 assert (ContLC K) by auto;
 apply HRed in H; auto.
-apply SN_step with (M:=ContAppl K M); auto.
+apply WT_step with (M:=ContAppl K M); auto.
 apply Step_KApplStep; auto.
 Qed.
 
-Lemma SN_N_SN_here:
+Lemma WT_N_WT_here:
 forall N,
-  SN N -> SN (here_LF N).
+  WT N -> WT (here_LF N).
 intros; induction H; subst.
 constructor; constructor; auto.
-apply step_SN; intros.
+apply step_WT; intros.
 inversion H1; subst.
 apply H0 in H4; auto.
 Qed.
@@ -509,14 +1067,14 @@ Qed.
 Theorem reducibility_props:
 forall A M
   (H_lc_t: lc_t_LF M),
-  (Red M A -> SN M)
+  (Red M A -> WT M)
   /\
   (neutral_LF M -> (forall M', M |-> M' -> Red M' A) -> Red M A).
 assert (exists (x:var), x \notin \{}) as nn by apply Fresh; destruct nn; auto;
 induction A; intros; split; simpl in *.
 (* base type *)
 auto.
-intros; apply step_SN; auto.
+intros; apply step_WT; auto.
 (* arrow type *)
 intros.
 (* Create variable of type A1 *)
@@ -526,41 +1084,41 @@ unfold ok_Bg_LF; rew_concat; constructor;
 [rewrite Mem_nil_eq | constructor]; auto.
 apply Mem_here.
 assert (forall x, neutral_LF (hyp_LF x)) by (intros; constructor).
-assert (forall x, SN (hyp_LF x))
-  by (intros; apply step_SN; intros; inversion H3).
+assert (forall x, WT (hyp_LF x))
+  by (intros; apply step_WT; intros; inversion H3).
 assert (forall x, Red (hyp_LF (fte x)) A1).
   intros; apply IHA1; auto.
   constructor.
   intros; inversion H4.
 assert (forall x, Red (appl_LF M (hyp_LF (fte x))) A2).
 intros; eapply H0; auto; constructor.
-assert (forall x, SN (appl_LF M (hyp_LF (fte x)))).
+assert (forall x, WT (appl_LF M (hyp_LF (fte x)))).
 intros; eapply IHA2; eauto; constructor; auto; constructor.
 (* From strong_norm (appl_L M (hyp_L x)) w deduce strong_norm M w *)
-eapply SN_appl; auto; constructor; auto; constructor.
+eapply WT_appl; auto; constructor; auto; constructor.
 intros; apply IHA2; try constructor; auto; intros; simpl in *.
 inversion H2; subst; inversion H0; eapply H1; eauto.
 (* box type *)
-intros; apply SN_box.
+intros; apply WT_box.
 constructor; auto.
 apply IHA; [constructor | ]; auto.
 intros; apply IHA; try constructor; auto; intros;
 inversion H2; subst; [inversion H0 | ]; apply H1; auto.
 (* dia type *)
 intros.
-assert (SN (ContAppl (IdK A) M)).
+assert (WT (ContAppl (IdK A) M)).
 apply H0 with (B:=A).
 constructor.
 constructor.
 intros. simpl.
 apply IHA in H2.
-apply SN_N_SN_here; apply SN_N_SN_here; destruct H2; auto.
+apply WT_N_WT_here; apply WT_N_WT_here; destruct H2; auto.
 simpl in H1.
-apply SN_here.
+apply WT_here.
 constructor; auto.
 auto.
 intros.
-apply step_SN; intros; apply step_neutral_ContAppl in H5; auto;
+apply step_WT; intros; apply step_neutral_ContAppl in H5; auto;
 destruct H5; destruct H5;
 subst; apply H1 with B; auto.
 Grab Existential Variables.
@@ -570,7 +1128,7 @@ Qed.
 Lemma property_1:
 forall A M
   (H_lc: lc_t_LF M),
-  Red M A -> SN M.
+  Red M A -> WT M.
 intros; eapply reducibility_props; eauto.
 Qed.
 
@@ -877,11 +1435,11 @@ lc_t_LF N -> Red N A -> Red (here_LF N) (<*>A).
 intros; simpl in *; intros; apply H3; auto.
 Qed.
 
-Lemma SN_letdia:
+Lemma WT_letdia:
 forall K M N,
-  SN M ->
-  SN (ContAppl K ([M // bte 0]N)) ->
-  SN (ContAppl K (here_LF (letdia_LF (here_LF M) N))).
+  WT M ->
+  WT (ContAppl K ([M // bte 0]N)) ->
+  WT (ContAppl K (here_LF (letdia_LF (here_LF M) N))).
 Admitted.
 
 Theorem main_theorem:
@@ -894,9 +1452,9 @@ forall G Gamma M A,
     (forall a b c, Mem (a,b,c) L -> Red c b) ->
   forall K B,
     ContTyping K A B ->
-    ContReducible K A B ->
-    SN (ContAppl K (here_LF (SL L M))).
-intros G Gamma M A LC HT; induction HT; unfold ContReducible in *;
+    RedCont K A B ->
+    WT (ContAppl K (here_LF (SL L M))).
+intros G Gamma M A LC HT; induction HT; unfold RedCont in *;
 intros.
 (* hyp *)
 assert (lc_t_LF (SL L (hyp_LF (fte v)))) by
@@ -920,7 +1478,7 @@ unfold open_LF in *.
 assert (exists x, x \notin L \u used_vars_te_LF (SL L0 M) \u
        from_list (map fst_ (map fst_ L0)) \u FV_L L0) by apply Fresh;
 destruct H6.
-assert (SN (ContAppl K (here_LF (SL L0 [hyp_LF (fte x) // bte 0]M)))).
+assert (WT (ContAppl K (here_LF (SL L0 [hyp_LF (fte x) // bte 0]M)))).
 apply H0 with B0; eauto.
 apply lc_t_subst_t_LF_bound; [constructor | inversion LC]; auto.
 rewrite <- H1.
@@ -993,7 +1551,7 @@ forall G Gamma M A,
   Red M A ->
   forall K B,
     ContTyping K A B ->
-    SN (ContAppl K (here_LF M)).
+    WT (ContAppl K (here_LF M)).
 Admitted.
 
 Lemma non_trivial:
@@ -1002,7 +1560,7 @@ forall G Gamma M A,
   G |= Gamma |- M ::: A ->
   forall K B,
     ContTyping K A B ->
-    SN (ContAppl K (here_LF M)).
+    WT (ContAppl K (here_LF M)).
 Admitted.
 *)
 
@@ -1010,7 +1568,7 @@ Admitted.
 forall G Gamma M A,
   lc_t_LF M ->
   G |= Gamma |- M ::: A ->
-  forall K B, ContTyping K A B -> SN (ContAppl K (here_LF M)).
+  forall K B, ContTyping K A B -> WT (ContAppl K (here_LF M)).
 intros G Gamma M A LC HT; induction HT; intros.
 *)
 
@@ -1045,14 +1603,14 @@ specialize H0 with x; apply H0 in H2;
 apply lc_t_n_LF_subst_t in H2; auto; constructor.
 Qed.
 
-Theorem SN_Lang:
+Theorem WT_Lang:
 forall G M A,
   emptyEquiv_LF G |= nil |- M ::: A ->
-  SN M.
+  WT M.
 intros.
 assert (lc_t_LF M).
   apply types_LF_lc_t_LF in H; auto.
-assert (SN (ContAppl (IdK A) (here_LF M))).
+assert (WT (ContAppl (IdK A) (here_LF M))).
 apply less_trivial_1 with (L:=nil) (K:=IdK A) (B:=A) in H; auto.
 rewrite SL_nil in H; auto.
 rew_concat; rew_map; clear M A H H0;
@@ -1060,9 +1618,9 @@ induction G; simpl; rew_concat; auto.
 intros; rewrite Mem_nil_eq in *; contradiction.
 intros; rewrite Mem_nil_eq in *; contradiction.
 constructor.
-unfold ContReducible; intros; simpl.
-repeat apply SN_N_SN_here; apply property_1 with (A:=A); auto.
-simpl in H1; apply SN_here; [constructor |]; auto; apply SN_here; auto;
+unfold RedCont; intros; simpl.
+repeat apply WT_N_WT_here; apply property_1 with (A:=A); auto.
+simpl in H1; apply WT_here; [constructor |]; auto; apply WT_here; auto;
 constructor; constructor; auto.
 Qed.
 *)
